\documentclass{article}
\usepackage{amsmath,amssymb}

\begin{document}


\begin{subequations}
    \begin{alignat}{3}
        & \min & \quad & \sum_{(o,t)\in \Theta} \sum_{e \in IE(t)}  f_e^{(o,t)} \cdot d_{(o,t)} \cdot r_{(o,t,i)} - \sum_{e'\in E} u_{e'}\cdot c_{e'} \hspace{126pt}    \label{eq:FullCooperationA} \\
    \end{alignat}

    \begin{alignat}{3}
        & \text{subject to}       & \sum_{e \in IE(z)} f_e^{(o,t,i)}-\sum_{e' \in OE(z)} f_{e'}^{(o,t,i)} & = 0, && \forall\ z\in V\setminus\{o,t\},\ \forall (o,t,i)\in\Theta, \label{eq:FullCooperationB}\\
        &                         & \sum_{e \in OE(o)} f_e^{(o,t,i)}                                    & \leq 1, && \forall\ (o,t,i)\in \Theta, \label{eq:FullCooperationC} \\
        &                         & \sum_{e \in OE(t)} f_e^{(o,t,i)}                                    & = 0, && \forall\ (o,t,i)\in \Theta, \label{eq:FullCooperationD} \\
        &                         & \sum_{(o,t,i) \in \Theta} f_e^{(o,t,i)}\cdot d_{(o,t,i)}            & \leq u_e\cdot q_{(o,t,i)}, &&  \forall\ e \in E, \label{eq:FullCooperationE}  \\
        &                         & \sum_{v \in S} \sum_{w \in S} f_{(v,w)}^{(o,t,i)}                   & \leq |S| -1, && \forall\; S \subset V,\ \forall\; (o,t,i) \in \Theta, \label{eq:FullCooperationF} \\
        &                         & f_e^{(o,t,i)}                                                       & \in \{0,1\}, &&  \forall\ e \in E,\ \forall (o,t,i)\in \Theta, \label{eq:FullCooperationG} \\
        &                         & u_e                                                                 & \in \{0,1\}, && \forall\; e \in E \\
        &                         & \sum_{(o,t,i)\in \Theta}\left[\sum_{e \in OE(o)} f_e^{(o,t,i)}\cdot d_{(o,t,i)}\cdot r_{(o,t,i)}\right. - & &&\nonumber \\
        &                         & - \left. \sum_{\substack{e=(w,w,j) \in E\colon\\j\not = i }} f_e^{(o,t,i)}\cdot d_{(o,t,i)}\cdot \frac{c_w}{q_e}\right] + & &&\nonumber \\
        &                         & + \sum_{\substack{(o,t,k)\in \Theta \colon \\ k \not = i}} \sum_{e=(v,w,i) \in E} f_e^{(o,t,k)}\cdot d_{(o,t,k)}\cdot \frac{c_e}{q_e} - & &&\nonumber  \\
        &                         & - \sum_{e=(v,w,i)\in E} c_e \cdot u_e & \geq min\_payoff[i] && 
    \end{alignat}

\end{subequations}

\end{document}